\documentclass{article} % This command is used to set the type of document you are working on such as an article, book, or presenation

\usepackage{geometry} % This package allows the editing of the page layout
\usepackage{amsmath}  % This package allows the use of a large range of mathematical formula, commands, and symbols
\usepackage{graphicx}  % This package allows the importing of images
\usepackage{soul}
\usepackage{amsfonts}
\usepackage{dirtytalk}
\usepackage{tabto}
\usepackage{xcolor,colortbl, amssymb}
\usepackage{forest}

% https://www.messletters.com/en/big-text/

\newcommand{\question}[2][]{\begin{flushleft}
        \textbf{Question #1}: \textit{#2}

\end{flushleft}}

\definecolor{Green}{rgb}{0, 1, 0}
\definecolor{Pink}{rgb}{1, .753, .796}

\newcommand{\sol}{\textbf{Solution}:} %Use if you want a boldface solution line
%\newcommand\tab[1][0.4cm]{\hspace*{#1}}
\newcommand{\maketitletwo}[2][]{\begin{center}
        \Large{\textbf{Homework #1}
            
            CMPSC 465} % Name of course here
        \vspace{5pt}
        
        \normalsize{Kinner Parikh  % Your name here
        
        \today}        % Change to due date if preferred
        \vspace{40pt}

        \text{I did not work in a group}

        \text{I did not consult without anyone my group member}

        \text{I did not consult any non-class materials}
        \newpage
        
\end{center}}
\begin{document}
    \maketitletwo[1]  % Optional argument is assignment number
    %Keep a blank space between maketitletwo and \question[1]
    
    \question[1]{In each of the following situations, indicate whether $f = O(g)$, or $f = \Omega(g)$,
     or both (in which case $f = \Theta(g)$). Give a one sentence justification for each of your answers.}

    a) $f(n) = n^{1.5}$, $g(n) = n^{1.3} \rightarrow \underline{f = \Omega(g)}$ and not $O(g)$ 
    because the exponent of $f$ is greater than 
    \tabto{27pt} the exponent in $g$. 
    
    \vspace{5pt}

    b) $f(n) = 2^{n-1}$, $g(n) = 2^n \rightarrow \underline{f = \Theta(g)}$ 
    because $f(n) = \frac{1}{2} \cdot 2^n$, and since we disregard the 
    \tabto{28pt} coefficient, we know that asymptotically $f$ is $2^n$, which is equivalent to $g$.

    \vspace{5pt}

    c) $f(n) = n^{1.3 \text{log}(n)}$, $g(n) = n^{1.5} \rightarrow \underline{f = \Omega(g)}$ 
    because simply comparing the exponents shows 
    \tabto{27pt} that $f$'s exponent will grow faster than $g$'s because $f$'s exponent grows based on $n$ while $g$'s 
    \tabto{27pt} is constant.

    \vspace{5pt}

    d) $f(n) = 3^n$, $g(n) = n \cdot 2^n \rightarrow \underline{f = \Omega(g)}$ 
    because based on the rule of exponential functions for 
    \tabto{28pt} asymptotic growth, the larger the base of the exponent, the faster it will grow. Since $3 > 2$, 
    \tabto{28pt} $f$ will grow faster than $g$.

    \vspace{5pt}

    e) $f(n) = (\text{log}\ n)^{100}$, $g(n) = n^{0.1} \rightarrow \underline{f = O(g)}$ 
    because log($n$) grows slower than $n$, and since 
    \tabto{28pt} the function is dependent on the base of the exponent, $g$ will grow faster than $f$.

    \vspace{5pt}

    f) $f(n) = n$, $g(n) = (\text{log}\ n)^{\text{log log} n} \rightarrow \underline{f = O(g)}$ 
    because $g$ is an exponential function and $f$ is 
    \tabto{28pt} linear, thus $g$ will grow faster than $f$.

    \vspace{5pt}

    g) $f(n) = 2^n$, $g(n) = n! \rightarrow \underline{f = O(g)}$
    because factorial grows much faster than any exponential 
    \tabto{28pt} function.

    \vspace{5pt}

    h) $f(n) = \text{log}(e^n)$, $g(n) = n \text{log}n \rightarrow \underline{f = O(g)}$ 
    because we can simplify $f$ down to $n$log($e$). Since
    \tabto{28pt} log($e$) is a numerical value, we can drop it and see that $f$ is a linear function, thus grows
    \tabto{28pt} slower than $n$log$n$.

    \vspace{5pt}

    i) $f(n) = n + \text{log}n$, $g(n) = n + (\text{log}n)^2 \rightarrow \underline{f = \Theta(g)}$
    because $($log$n)^2$ grows slower than $n$, thus 
    \tabto{26pt} both $f$ and $g$ exhibit linear growth.

    \vspace{5pt}

    j) $f(n) = 5n + \sqrt{n}$, $g(n) = \text{log}n + n \rightarrow \underline{f = \Theta(g)}$
    because both $\sqrt{n}$ and log$n$ grow slower than 
    \tabto{26pt} linear growth, thus, both $f$ and $g$ exhibit linear growth.

    \newpage

    \question[2]{}
    
    a) Prove that $R(i) \geq  3^{i/2}\ \forall i \geq 2$ where $R(i) = R(i - 1) + R(i - 2) + R(i - 3) $
    \vspace{5pt}
    \tabto{28pt} Proof:
    \tabto{28pt} We proceed by induction on the variable $i$.
    \tabto{28pt} \textbf{Base Case} ($i = 2, 3, 4$):
    \tabto{28pt} $R(2) = 3$ and $3^{2/2} = 3$, thus the case holds
    \tabto{28pt} $R(3) = R(2) + R(1) + R(0) = 3+2+1=6$ and $3^{3/2} \approx 5.196$, thus the case holds
    \tabto{28pt} $R(4) = R(3) + R(2) + R(1) = 6+3+2=11$ and $3^{4/2} = 9$, thus the case holds
    
    \vspace{5pt}

    \tabto{28pt} \textbf{Inductive Hypothesis} ($i = n$): 
    \tabto{28pt} For any arbitrary positive integer $i = n$ where $n \geq 2$, assume that $R(n) \geq 3^{n/2}$ 
    \tabto{28pt} This means that $R(n - 1) + R(n - 2) + R(n - 3) \geq 3^{n/2}$

    \vspace{5pt}

    \tabto{28pt} \textbf{Inductive Step} ($i = n + 1$): 
    \tabto{28pt} We have to show that $R(n + 1) \geq 3^{(n + 1)/2}$
    \tabto{28pt} Expanding this, we get $R(n) + R(n - 1) + R(n - 2) \geq 3^{(n + 1)/2}$
    \tabto{28pt} From the inductive hypothesis, we know that $R(n), R(n - 1), R(n - 2)$ holds.
    \tabto{28pt} Plugging this in, we can say that $R(n + 1) \geq 3^{0.5n} + 3^{0.5n - 0.5} + 3^{0.5n - 1}$
    \tabto{217pt} = $3^{0.5n}(1 + 3^{-0.5} + 3^{-1})$
    \tabto{217pt} = $3^{0.5n}(\frac{3+4\sqrt3}{3\sqrt3})$
    \tabto{217pt} = $3^{0.5n}(1.911)$
    \tabto{28pt} So, $R(n + 1) \geq 3^{0.5n}(1.911) \geq 3^{0.5n}(\sqrt3)$
    \tabto{28pt} Since $1.911 > \sqrt3$, the statement $R(n + 1) \geq 3^{(n + 1)/2}$ holds.
    \tabto{28pt} Therefore, $R(i) \geq  3^{i/2}\ \forall i \geq 2.\ \square$

    \vspace{5pt}

    b) Recursion Tree

    \begin{forest}
        [$R(i)$
            [$R(i - 1)$[$R(i - 2)$][$R(i - 3)$][$R(i - 4)$]]
            [$R(i - 2)$[$R(i - 3)$][$R(i - 4)$][$R(i - 5)$]]
            [$R(i - 3)$[$R(i - 4)$][$R(i - 5)$][$R(i - 6)$]]]
    \end{forest}

    \newpage

    \question[3]{Prove that $O_1(g(n)) = O_2(g(n))\ \forall g$}

    $O_1(g(n)) = \{f(n): \exists c_1, n_0 > 0 \text{ s.t. }f(n) \leq c_1g(n), \forall n \geq n_0\}$
    
    $O_2(g(n)) = \{f(n): \exists c_2 >0 \text{ s.t. } f(n) \leq c_2g(n), \forall n > 0\}$


\end{document}
